theories/prob_eff_lang/probblaze/examples/DH_KE/new_schan_ri.v
@@ -1,0 +1,275 @@
+From iris.proofmode Require Import base proofmode classes.                  
+From iris.base_logic.lib Require Import  na_invariants.  
+From iris.algebra Require Import agree excl auth frac excl_auth.
+From iris.algebra.lib Require Import dfrac_agree.
+From clutch Require Import stdpp_ext.
+From clutch.prob_eff_lang.probblaze Require Import logic primitive_laws proofmode
+  spec_rules spec_ra 
+  class_instances.
+From clutch.prob_eff_lang.probblaze Require Import tactics.
+From clutch.prob_eff_lang.probblaze Require Import def_dhke.
+From clutch.prob_eff_lang.probblaze Require Import dhke_channel.
+(*From clutch.prob_eff_lang.probblaze Require Import def_schannel.*)
+From clutch.prob_eff_lang.probblaze Require Import sem_types sem_row sem_sig sem_judgement sem_def.
+From clutch.prob_eff_lang.probblaze Require Import p_composition.
+From clutch.prob_eff_lang.probblaze Require Import newdef_schan.
+
+Import fingroup.
+
+Import fingroup.fingroup.
+
+(*Import valgroup_notation.*)
+Import valgroup_tactics.
+
+
+Section schan_security.
+  Context `{probblazeRGS Σ}.
+  Context {vg: val_group}.
+  Context {cg: clutch_group_struct}.
+  Context {G : clutch_group (vg:=vg) (cg:=cg)}.
+  Context {vgg : @val_group_generator vg}.
+  Context `{!inG Σ (exclR unitO), !inG Σ dfracO, !inG Σ (dfrac_agreeR valO)}.
+
+
+  Definition REAL_CHAN : val :=
+    λ: "f" "doLeakSend" "doLeakRecv" "doKeyLeak",  
+      effect "channel"
+      let: "doSend" := (λ: "m", do: (EffName "channel") (Send "m")) in
+      let: "doRecv" := (λ: "m", do: (EffName "channel") (Recv "m")) in
+      (*effect "schannel"
+      let: "doSecSend" := (λ: "m", do: (EffName "schannel") (Send "m")) in
+      let: "doSecRecv" := (λ: "m", do: (EffName "schannel") (Recv "m")) in *)
+      effect "getKey"
+      let: "doGK" := (λ: "party", do: (EffName "getKey") "party") in
+      F_OAUTH "channel" "doSend" "doRecv" (F_KE_L "getKey" "doGK" "f" "doKeyLeak") "doLeakSend" "doLeakRecv".  
+
+  Definition atokN' : namespace := nroot .@ "atokN1".
+  Definition btokN' : namespace := nroot .@ "btokN1".
+
+   (*Theories for the interaction of the secure channel with the environment*)
+  (*-------------------------------------------------------------*)
+
+  (* Theories for the authenticated channel leaks *)
+  (*-------------------------------------------------------------*)
+   (* Send TO Bob*)
+   Program Definition LASendBob (leakauth1 leakauth2 : label) : iThy Σ :=
+  λ e1 e2, (λne Q,
+              ∃ m1 m2 : val,
+                ⌜e1 = (do: leakauth1 (SendV (m1, bob)))⌝%E ∗ 
+                           ⌜ e2 = do: leakauth2 (SendV (m2, bob)) ⌝%E ∗
+                                      □ Q (Val #()%V) (Val #()%V))%I.
+  Next Obligation. solve_proper. Qed.
+  (* Send TO Alice*)
+  Program Definition LASendAlice (leakauth1 leakauth2 : label) : iThy Σ :=
+  λ e1 e2, (λne Q,
+              ∃ m1 m2 : val,
+                ⌜e1 = (do: leakauth1 (SendV (m1, alice)))⌝%E ∗ 
+                           ⌜ e2 = do: leakauth2 (SendV (m2, alice)) ⌝%E ∗
+                                      □ Q (Val #()%V) (Val #()%V))%I.
+  Next Obligation. solve_proper. Qed.
+  (*Recv FROM bob*) 
+  Program Definition LARecvBob (leakauth1 leakauth2 : label) : iThy Σ :=
+   λ e1 e2, (λne Q,
+                ⌜ e1 = do: leakauth1 (RecvV bob) ⌝%E ∗
+                ⌜ e2 = do: leakauth2 (RecvV bob) ⌝%E ∗
+                □ ((∀ b1 b2 : nat, Q (SOMEV #b1) (SOMEV #b2)) ∧ Q NONEV NONEV)
+             )%I.
+  Next Obligation. solve_proper. Qed.
+ (* Recv FROM Alice *)
+  Program Definition LARecvAlice (leakauth1 leakauth2 : label) : iThy Σ :=
+     λ e1 e2, (λne Q,
+                ⌜ e1 = do: leakauth1 (RecvV alice) ⌝%E ∗
+                ⌜ e2 = do: leakauth2 (RecvV alice) ⌝%E ∗
+                □ ((∀ b1 b2 : nat, Q (SOMEV #b1) (SOMEV #b2)) ∧ Q NONEV NONEV)
+             )%I.
+  Next Obligation. solve_proper. Qed.
+
+  
+  (* Theories for the key exchange leaks*)
+  (*---------------------------------------------------------*)
+  (*Send TO Alice*)
+  Program Definition KLeakSendAlice (keyleak1 keyleak2 : label) : iThy Σ :=
+    λ e1 e2, (λne Q,
+                ⌜ e1 = do: keyleak1 (SendV alice) ⌝%E ∗
+                           ⌜ e2 = do: keyleak2 (SendV alice) ⌝%E ∗
+                                      □ Q (Val #()%V) (Val #()%V))%I.
+  Next Obligation. solve_proper. Qed.
+  (* Send TO Bob *)
+  Program Definition KLeakSendBob (keyleak1 keyleak2 : label) : iThy Σ :=
+    λ e1 e2, (λne Q,
+                ⌜ e1 = do: keyleak1 (SendV bob) ⌝%E ∗
+                           ⌜ e2 = do: keyleak2 (SendV bob) ⌝%E ∗
+                                      □ Q (Val #()%V) (Val #()%V))%I.
+  Next Obligation. solve_proper. Qed.
+
+
+  (*Program Definition KLeakRecvAlice : iThy Σ :=
+    λ e1 e2, (λne Q,
+                ⌜ e1 = do: keyleak1 (RecvV alice) ⌝%E ∗
+                           ⌜ e2 = do: keyleak2 (RecvV alice) ⌝%E ∗
+                                      □ Q (Val #()%V) (Val #()%V))%I.
+  Next Obligation. solve_proper. Qed.*) 
+  (* Recv FROM Alice *)
+   Program Definition KLeakRecvAlice (keyleak1 keyleak2 : label) : iThy Σ :=
+    λ e1 e2, (λne Q,
+                ⌜ e1 = do: keyleak1 (RecvV alice) ⌝%E ∗
+                           ⌜ e2 = do: keyleak2 (RecvV alice) ⌝%E ∗
+                                      □ (Q NONEV NONEV ∗ Q (SOMEV #0) (SOMEV #0)))%I.
+  Next Obligation. solve_proper. Qed.
+ (* Recv FROM Bob *)
+  Program Definition KLeakRecvBob (keyleak1 keyleak2 : label) : iThy Σ :=
+    λ e1 e2, (λne Q,
+                ⌜ e1 = do: keyleak1 (RecvV bob) ⌝%E ∗
+                           ⌜ e2 = do: keyleak2 (RecvV bob) ⌝%E ∗
+                                      □ (Q NONEV NONEV ∗ Q (SOMEV #0) (SOMEV #0)))%I.
+  Next Obligation. solve_proper. Qed.
+  
+  (* Theories relating the authenticated channel with the secure channel leak*)
+  (*-----------------------------------------------------------------------------*)
+  Program Definition SendALSAlice (channel leaksec : label) : iThy Σ :=
+    λ e1 e2, (λne Q,
+                ∃ m : val,
+                  (⌜ e1 = do: channel (SendV (m, alice)) ⌝%E ∗
+                  ⌜  e2 = do: leaksec (SendV alice)⌝%E) ∗ □ (Q (Val #()%V) (Val #()%V)))%I.
+  Next Obligation. solve_proper. Qed.
+
+  Program Definition SendALSBob (channel leaksec : label) : iThy Σ :=
+    λ e1 e2, (λne Q,
+                ∃ m : val,
+                  (⌜ e1 = do: channel (SendV (m, bob)) ⌝%E ∗
+                  ⌜  e2 = do: leaksec (SendV bob)⌝%E) ∗ □ (Q (Val #()%V) (Val #()%V)))%I.
+  Next Obligation. solve_proper. Qed. 
+
+  Program Definition RecvALSAlice (channel leaksec : label) : iThy Σ :=
+    λ e1 e2, (λne Q,
+                  (⌜ e1 = do: channel (RecvV alice) ⌝%E ∗
+                  ⌜  e2 = do: leaksec (RecvV alice)⌝%E) ∗ □ (Q (Val #()%V) (Val #()%V)))%I.
+  Next Obligation. solve_proper. Qed.    
+
+  Program Definition RecvALSBob (channel leaksec : label) : iThy Σ := 
+    λ e1 e2, (λne Q,
+                  (⌜ e1 = do: channel (RecvV bob) ⌝%E ∗
+                  ⌜  e2 = do: leaksec (RecvV bob)⌝%E) ∗ □ (Q (Val #()%V) (Val #()%V)))%I.
+  Next Obligation. solve_proper. Qed.  
+
+  (*Program Definition ChanLeakSec : iThy Σ := iThySum (iThySum SendALSAlice SendALSBob) (iThySum RecvALSAlice RecvALSBob). *)
+(*  Program Definition ChanLeakSec : iThy Σ := (iThySum SendALSAlice RecvALSBob).
+  
+  Definition LblEnvSec := [ ([channel; getKey1; schannel1], [leaksec; schannel2; getKey2], iThyBot)    ;
+                            ([keyleak1], [keyleak2],iThySum (iThySum KLeakSendAlice KLeakRecvAlice) (iThySum KLeakSendBob KLeakRecvBob));
+                            ([leakauth1], [leakauth2], iThySum (iThySum LASendAlice LASendBob) (iThySum LARecvAlice LARecvBob))].
+
+   Definition LblEnvSec' := [ ([leaksec; getKey1; schannel1], [channel; schannel2; getKey2], iThyBot)    ;
+                            ([keyleak1], [keyleak2],iThySum (iThySum KLeakSendAlice KLeakRecvAlice) (iThySum KLeakSendBob KLeakRecvAlice));
+                            ([leakauth1], [leakauth2], iThySum (iThySum LASendAlice LASendBob) (iThySum LARecvAlice LARecvBob))].
+*)
+
+  (*Theories relating the secure channel effects for the client*)
+  (*---------------------------------------------------------*)
+  Program Definition SendSecBob (schannel1 schannel2 : label) : iThy Σ :=
+     λ e1 e2, (λne Q,
+                ∃ m m': val, 
+                            (⌜ e1 = do: schannel1 (SendV (m, alice)) ⌝%E ∗
+                             ⌜ e2 = do: schannel2 (SendV (m', alice)) ⌝%E)  ∗ 
+                            □ (Q (Val #()%V) (Val #()%V))
+             )%I.
+  Next Obligation. solve_proper. Qed.
+  
+  
+   (*Program Definition SendSecBobImpl γtok γfrac γsec ℓ : iThy Σ :=
+     λ e1 e2, (λne Q,
+                ∃ m m': val, ((|={⊤, ⊤ ∖ ↑ℓ }=> ((own γfrac DfracDiscarded -∗ (|={⊤ ∖ ↑ℓ, ⊤}=> token γtok ∗ own γsec (to_dfrac_agree DfracDiscarded m) ∗ ⌜m = m'⌝)) ∨ |={⊤ ∖ ↑ℓ , ⊤}=> own γfrac DfracDiscarded)) ∗  
+                            (⌜ e1 = do: schannel1 (SendV (m, alice)) ⌝%E ∗
+                             ⌜ e2 = do: schannel2 (SendV (m', alice)) ⌝%E)  ∗ 
+                            □ (Q (Val #()%V) (Val #()%V)))
+             )%I.
+  Next Obligation. solve_proper. Qed.*)
+  
+  Program Definition SendSecAlice (schannel1 schannel2 : label) : iThy Σ :=
+     λ e1 e2, (λne Q,
+                ∃ m m' : val,   
+                             (⌜ e1 = do: schannel1 (SendV (#0, bob)) ⌝%E ∗
+                              ⌜ e2 = do: schannel2 (SendV (#0, bob)) ⌝%E)  ∗ 
+                             □ (Q (Val #()%V) (Val #()%V))
+             )%I.
+  Next Obligation. solve_proper. Qed.
+
+   (* Program Definition SendSecAliceImpl γtok γfrac γsec ℓ : iThy Σ :=
+     λ e1 e2, (λne Q,
+                ∃ m m' : val, ((|={⊤, ⊤ ∖ ↑ℓ }=> ((own γfrac DfracDiscarded -∗ (|={⊤ ∖ ↑ℓ, ⊤}=> token γtok ∗ own γsec (to_dfrac_agree DfracDiscarded m) ∗ ⌜m = m'⌝)) ∨ |={⊤ ∖ ↑ℓ , ⊤}=> own γfrac DfracDiscarded)) ∗  
+                             (⌜ e1 = do: schannel1 (SendV (m, bob)) ⌝%E ∗
+                              ⌜ e2 = do: schannel2 (SendV (m', bob)) ⌝%E)  ∗ 
+                             □ (Q (Val #()%V) (Val #()%V)))
+             )%I.
+  Next Obligation. solve_proper. Qed.*)
+  
+  Program Definition RecvSecBob (schannel1 schannel2 : label) : iThy Σ :=
+     λ e1 e2, (λne Q,
+                ⌜ e1 = do: schannel1 (RecvV bob) ⌝%E ∗
+                ⌜ e2 = do: schannel2 (RecvV bob) ⌝%E ∗
+                □ (Q NONEV NONEV)
+             )%I.
+  Next Obligation. solve_proper. Qed. 
+    
+  Program Definition RecvSecAlice (schannel1 schannel2 : label) : iThy Σ :=
+     λ e1 e2, (λne Q,
+                 ⌜ e1 = do: schannel1 (RecvV alice) ⌝%E ∗
+                 ⌜ e2 = do: schannel2 (RecvV alice) ⌝%E ∗
+                 □ (Q NONEV NONEV )
+             )%I.
+  Next Obligation. solve_proper. Qed.
+
+
+   (* semantic types*)
+  (*----------------------------------------------------------------------------*)
+
+   Definition sem_ty_group : sem_ty Σ := (λ v1 v2, ∃ g : vgG, ⌜ v1 = g ⌝ ∗ ⌜ v2 = g ⌝)%I.
+  Notation "'𝔾'" := sem_ty_group. 
+  (*Program Definition bot_mono := {| pmono_prot_car := iThyBot ; pmono_prot_prop := _ |}.
+  Next Obligation. solve_proper. Defined.
+ 
+  Definition thy_sec_chan (l1 l2 : label) := @SemSig Σ bot_mono (l1,l2).
+  Program Definition thy_sec_row (channel leaksec getKey1 getKey2 schannel1 schannel2 : label) :=
+    SemRow [([channel; getKey1; schannel1] , [leaksec; getKey2; schannel2] , bot_mono)] _.*)
+  Program Definition keyleak_mono (keyleak1 keyleak2 : label) := {| pmono_prot_car := iThySum (iThySum (KLeakSendAlice keyleak1 keyleak2) (KLeakRecvAlice keyleak1 keyleak2)) (iThySum (KLeakSendBob keyleak1 keyleak2) (KLeakRecvBob keyleak1 keyleak2)) ; pmono_prot_prop := _|}.
+  Next Obligation.
+   iIntros (????).
+   iIntros (??) "#HΦ [[HS | HR] | [HS | HR]]".
+   1: iLeft; iLeft. 2: iLeft; iRight. 3: iRight; iLeft. 4: iRight; iRight.
+   1,3 : iDestruct "HS" as (??) "#H"; simpl; iSplit; first done; iSplit; first done; iModIntro; by iApply "HΦ".
+   all: iDestruct "HR" as (??) "(#H1 & #H2)"; simpl; iSplit; first done; iSplit; first done; iModIntro; iSplitL " "; iApply "HΦ"; try (iApply "H1"); try (iApply "H2").
+  Qed.
+  Definition keyleak (keyleak1 keyleak2 : label) := @SemSig Σ (keyleak_mono keyleak1 keyleak2) (keyleak1, keyleak2).
+  Lemma keyleak_pers_mono_row (channel leaksec getKey1 getKey2 schannel1 schannel2 keyleak1 keyleak2 : label) : ⊢ pers_mono_row (iLblSig_to_iLblThy [([channel; getKey1; schannel1; keyleak1] , [leaksec; getKey2; schannel2; keyleak2] , keyleak keyleak1 keyleak2)]).
+  Proof. Admitted.
+  Definition keyleak_row (channel leaksec getKey1 getKey2 schannel1 schannel2 keyleak1 keyleak2 : label) := SemRow [([channel; getKey1; schannel1; keyleak1] , [leaksec; getKey2; schannel2; keyleak2] , keyleak keyleak1 keyleak2)] (keyleak_pers_mono_row channel leaksec getKey1 getKey2 schannel1 schannel2 keyleak1 keyleak2).
+ 
+  Program Definition leakauth_mono (leakauth1 leakauth2 : label) := {| pmono_prot_car := iThySum (iThySum (LASendAlice leakauth1 leakauth2) (LASendBob leakauth1 leakauth2)) (iThySum (LARecvAlice leakauth1 leakauth2) (LARecvBob leakauth1 leakauth2)) ; pmono_prot_prop := _ |}.
+  Next Obligation.
+    iIntros (??????) "#HΦ [[HS | HS] | [HR | HR]]".
+    1: iLeft; iLeft. 2: iLeft; iRight. 3: iRight; iLeft. 4: iRight; iRight.
+    1,2 : iDestruct "HS" as (??) "(#H1 & #H2 & #H3)"; simpl; iExists m1, m2; iSplit; first done; iSplit; first done;
+                                                                         iModIntro; by iApply "HΦ". 
+    all : iDestruct "HR" as "(#H1 & #H2 & #H3)"; simpl; iSplit; first done; iSplit; first done; iModIntro;
+    iDestruct "H3" as "[Hs Hn]"; iSplitL " "; try (iIntros (??)); iApply "HΦ"; try (iApply "Hs"); try (iApply "Hn").
+  Qed.
+
+  Definition leakauth (leakauth1 leakauth2 : label) := @SemSig Σ (leakauth_mono leakauth1 leakauth2) (leakauth1, leakauth2).
+  Lemma leakauth_pers_mono_row (leakauth1 leakauth2 : label) : ⊢ pers_mono_row (iLblSig_to_iLblThy [([leakauth1], [leakauth2], leakauth leakauth1 leakauth2)]).
+  Proof. Admitted.
+  Definition leakauth_row (leakauth1 leakauth2 : label) := SemRow [([leakauth1],[leakauth2] , leakauth leakauth1 leakauth2 )] (leakauth_pers_mono_row leakauth1 leakauth2).
+  Program Definition envsec_row (channel leaksec getKey1 getKey2 schannel1 schannel2 keyleak1 keyleak2 leakauth1 leakauth2 : label) :=
+    sem_row_union (keyleak_row channel leaksec getKey1 getKey2 schannel1 schannel2 keyleak1 keyleak2) (leakauth_row leakauth1 leakauth2).
+
+(*Verification of F_OAUTH[F_KE_L[CHAN[]]] ≤ CHAN_SIM[F_CHAN[]]*)
+(*----------------------------------------------------------*)
+Lemma F_KE_CHAN_SIM (f1 f2 : val) (L : sem_row Σ) :
+    sem_val_typed f1 f2 ((∀ᵣ θₕ, ((sem_ty_sum 𝟙 𝟙) -{ θₕ }-> (Option  𝔾)) -{ θₕ }-> ((sem_ty_sum 𝟙 𝟙) -{ θₕ }-> (Option  𝔾)) -{ sem_row_union  θₕ L }-> 𝟙))%T -∗ 
+    BREL REAL_CHAN (CHAN f1)
+      ≤ CHAN_SIM (F_CHAN f2) <|⊥|> {{λ v1 v2,
+                                       ∀ (channel leaksec getKey1 getKey2 schannel1 schannel2 leakauth1 leakauth2 keyleak1 keyleak2 : label),
+                                       BREL v1 (λ: "m", do: leakauth1 (Send "m"))%V (λ: "m", do: leakauth1 (Recv "m"))%V (λ: "m", do: keyleak1 "m")%V (λ: <>, #())%V ≤ v2 (λ: "m", do: keyleak2 "m")%V (λ: "m", do: leakauth2 (Send "m"))%V (λ: "m", do: leakauth2 (Recv "m"))%V <| (iLblSig_to_iLblThy (envsec_row channel leaksec getKey1 getKey2 schannel1 schannel2 leakauth1 leakauth2 keyleak1 keyleak2 )) ++ (iLblSig_to_iLblThy L) |> {{ (λ w1 w2, 𝟙%T w1 w2)}}}}.
+Proof.
+Admitted.
+ 
+End schan_security.
