theories/prob_eff_lang/probblaze/examples/DH_KE/newdef_schan.v
@@ -1,0 +1,218 @@
+(*From iris.proofmode Require Import base proofmode classes.
+From iris.base_logic.lib Require Import na_invariants.
+From iris.algebra Require Import agree excl auth frac excl_auth.
+From iris.algebra.lib Require Import dfrac_agree.
+From clutch Require Import stdpp_ext.
+From clutch.prob_eff_lang.probblaze Require Import logic primitive_laws proofmode
+ spec_rules spec_ra class_instances.
+From clutch.prob_eff_lang.probblaze Require Import tactics.
+From clutch.prob_eff_lang.probblaze Require Import sem_types sem_row sem_sig sem_judgement sem_def.*)
+From clutch.prob_eff_lang.probblaze Require Export notation valgroup p_composition.
+From clutch.prob_eff_lang.probblaze Require Export def_dhke.
+
+Import fingroup.
+
+Import fingroup.fingroup.
+
+Import valgroup_notation.
+Import valgroup_tactics.
+
+Section schannel.
+  Context {vg : val_group}.
+  Context {cg : clutch_group_struct}.
+  Context {vgg : @val_group_generator vg}.
+  (*Context (channel leaksec getKey1 getKey2 leakauth1 leakauth2 schannel1 schannel2 : label).*)
+
+  #[local] Notation n := (S n'').
+
+
+   Definition F_OAUTH : val :=
+    λ: "channel" "doSend" "doRecv" "f" "doLeakSend" "doLeakRecv",
+      let: "message" := ref NONEV in
+      (*effect "channel"
+      let: "doSend" := (λ: "m", do: (EffName "channel") (Send "m")) in
+      let: "doRecv" := (λ: "m", do: (EffName "channel") (Recv "m")) in*)
+      handle: "f" "doSend" "doRecv" with
+      | effect (EffName "channel") "payload", rec "k" as multi =>
+      match: "payload" with
+      (*Send Auth*)
+      | InjL "payload" =>
+          let, ("m", "dst") := "payload" in
+          match: !"message" with
+          | NONE => "message" <- SOME "m" ;;
+                   ("doLeakSend" ("m", "dst"));; "k" #()%V
+          | SOME "message" => "k" #()%V
+          end
+      (* Receive Auth *)
+      | InjR "from" => 
+          let: "r" := ("doLeakRecv" "from") in
+          match: "r" with
+          | NONE => "k" NONEV
+          | SOME "x" => "k" !"message"                         
+          end
+      end
+     | return "y" => #()%V
+    end.
+
+   (*placeholder for now*)
+  Definition xor (e1 e2 : expr) : val := #()%V.
+
+   Definition CHAN : val :=
+    λ: "f" "doSend" "doRecv" "doGK",
+      let: "message" := ref NONEV in
+      effect "schannel"
+      let: "doSecSend" := (λ: "m", do: (EffName "schannel") (Send "m")) in
+      let: "doSecRecv" := (λ: "m", do: (EffName "schannel") (Recv "m")) in
+      handle: "f" "doSecSend" "doSecRecv" with
+      | effect (EffName "schannel") "payload", rec "k" as multi =>
+        match: "payload" with
+          (*SendSecure*)
+        | InjL "payload" =>
+            let, ("m", "dst") := "payload" in
+            match: !"message" with
+              | NONE => "message" <- SOME "m";;
+                     let: "key" := "doGK" ("dst") in
+                                     match: "key" with
+                                     | NONE => "k" #()%V
+                                     | SOME "x" =>
+                                         let: "enc_m" := xor "x" "m" in
+                                         ("doSend" (Send ("enc_m", bob)));;
+                                         "k" #()%V
+                                     end
+              | SOME "m" => "k" #()%V
+               end
+          (*RecvSecure*)
+        | InjR "from" =>
+            let: "key" := "doGK" ("from") in
+                            match: "key" with
+                            | NONE => "k" NONEV
+                            | SOME "key" =>
+                                let: "r" := ("doRecv" (Recv "from")) in
+                                match: "r" with
+                                | NONE => "k" NONEV
+                                | SOME "x" =>
+                                    let: "enc_m" := xor "key" "x" in
+                                    "k" (SOME "enc_m")
+                                end       
+                            end                              
+        end
+      | return "y" => #()%V
+  end.
+  
+   (* Ideal functionality of the ONE-SHOT secure channel *)
+   Definition F_CHAN : val :=
+    λ: "f" "doLeakSend" "doLeakRecv",                           
+      let: "message" := ref NONEV in
+      effect "schannel"
+      let: "doSecSend" := (λ: "m", do: (EffName "schannel") (Send "m"))  in
+      let: "doSecRecv" := (λ: "m", do: (EffName "schannel") (Recv "m")) in
+      handle: "f" "doSecSend" "doSecRecv" with
+       | effect (EffName "schannel") "payload", rec "k" as multi =>
+        match: "payload" with
+          (*SendSecure*)
+         | InjL "payload" =>
+            let, ("m", "dst") := "payload" in
+            match: !"message" with
+            | NONE => "message" <- SOME "m";;
+                     ("doLeakSend" (Send ("dst")));;
+                     "k" #()%V 
+            | SOME "x" => "k" #()%V
+            end
+          (*ReceiveSecure*)
+         | InjR "from" =>
+            let: "r" := ("doLeakRecv" (Recv "from")) in
+            match: "r" with
+            | NONE => "k" NONEV
+            | SOME "x" => "k" (SOME "x")
+            end              
+         end
+       | return "y" => #()%V
+    end.
+
+    (*Simulator for the one message secure channel *)
+ (* Assumes a fixed direction from Alice to Bob *)       
+  Definition CHAN_SIM : val :=
+   λ: "f" "doKeyLeak" "doLeakASend" "doLeakARecv",                            
+    let: "α" := alloc #n in
+    let: "message" := ref NONEV in
+    effect "leaksec"
+    let: "doLeakSecSend" := (λ: "m", do: (EffName "leaksec") (Send "m")) in
+    let: "doLeakSecRecv" := (λ: "m", do: (EffName "leaksec") (Recv "m")) in
+    handle: "f" "doLeakSecSend" "doLeakSecRecv" with
+    | effect (EffName "leaksec") "payload", rec "k" as multi =>
+        match: "payload" with
+          (*Broadcast a message*)
+        | InjL "payload" =>
+            (* assuming "dst" is alice for now *)
+            (*let, ("m", "dst") := "payload" in*)
+            ("doKeyLeak" (Send("payload")));;
+            let: "r" := "doKeyLeak" (Recv bob) in
+                          match: "r" with
+                          | NONE =>
+                              "k" NONEV
+                          | SOME "x" =>
+                              match: !"message" with
+                              | NONE =>
+                                  let: "m'" := (samplelbl "α" #()%V) in
+                                  let: "mA" := g^"m'" in
+                                  "message" <- SOME "m'";;
+                                  ("doLeakASend" (Send ("mA", bob)));;
+                                  "k" #()%V
+                              | SOME "m" => "k" #()%V
+                              end    
+                          end                           
+                        | InjR "from" =>
+                            ("doKeyLeak" (Send "from"));;
+             let: "r" := "doKeyLeak" (Recv "from") in
+                           match: "r" with
+                           | NONE =>
+                               (*(do: leakauth ("from"));;*)
+                               "k" NONEV
+                           | SOME "x" =>
+                               (*(do: keyleak (Send (bob)));;*)
+                               let: "rla" := ("doLeakARecv" (Recv "from")) in
+                               match: "rla" with
+                               | NONE => "k" NONEV
+                               | SOME "x" => "k" !"message"
+                               end
+                                 
+                           end                             
+        end
+    | return "y" => "y" end.
+
+   Definition F_KE_L : val :=
+  λ: "getKey" "doGK" "f" "doKeyLeak",                           
+    (* Magically share a presampled key *)
+    let: "c" := (sample #()%V) in
+    let: "key" := g ^ "c" in
+   (* effect "getKey"
+    let: "doGK" := (λ: "party", do: (EffName "getKey") "party") in*)
+    handle: "f" "doGK" with
+    | effect (EffName "getKey") "p", rec "k" as multi =>
+        match: "p" with
+          (* Alice *)
+          InjL <> =>
+            (* Send a dummy value *)
+            ("doKeyLeak" (Send(bob)));;
+            (* Receive a dummy value *)
+            let: "r" := "doKeyLeak" (Recv bob) in
+            match: "r" with
+              NONE => "k" NONEV
+            | SOME "w" => "k" (SOME "key")
+            end
+        (* Bob  *)
+        | InjR <> =>
+            let: "r" := "doKeyLeak" (Recv alice) in
+            match: "r" with
+              NONE => "k" NONEV
+            | SOME "w" => 
+                ("doKeyLeak" (Send alice));;
+                "k" (SOME "key")
+            end
+       end
+    | return "y" => "y" end.
+
+
+  
+
+End schannel.
